src/Var.v
@@ -59,7 +59,9 @@ Arguments unshift_name n1 n2 : simpl nomatch.
 
 Definition Zero := Empty_set.
 
-Inductive Succ {S : Set} : Set := succ0 | succS (s : S).
+Inductive Succ (S : Set) : Set := succ0 | succS (s : S).
+Arguments succ0 {S}.
+Arguments succS {S} s.
 
 Fixpoint level (V : nat) : Set :=
   match V with
@@ -82,6 +84,172 @@ Fixpoint level_extend {V} : level V -> level (S V) :=
       end
   end.
 Arguments level_extend {V} !l.
+
+Fixpoint level_extend_by {N} V : level N -> level (N + V) :=
+  match N return level N -> level (N + V) with
+  | 0 => fun l => Empty_set_rec _ l
+  | S N =>
+    fun l =>
+      match l with
+      | succ0 => l0
+      | succS s => lS (@level_extend_by N V s)
+      end
+  end.
+Arguments level_extend_by {N} V !l.
+
+Fixpoint lSn N {V} : level V -> level (N + V) :=
+  fun l =>
+    match N with
+    | 0 => l
+    | S N => lS (lSn N l)
+    end.
+
+Definition is_succS {N} (l : level (S N)) :=
+  match l with
+  | succ0 => False
+  | succS _ => True
+  end.
+
+Definition discriminate_level {N} (l : level N) :
+  succ0 <> succS l :=
+  fun eql =>
+    eq_ind (succS l) is_succS I succ0 (eq_sym eql).
+
+Definition inv_succS {N} l1 (l2 : level (S N)) :=
+  match l2 with
+  | succS l2' => l1 = l2'
+  | succ0 => False
+  end.
+
+Definition injective_succS {N} (l1 l2 : level N) :
+  succS l1 = succS l2 -> l1 = l2 :=
+  fun eql =>
+    eq_ind (succS l1) (inv_succS l1) eq_refl (succS l2) eql.
+
+Definition level_one_eq {l1 l2 : level 1} : l1 = l2 :=
+  match l1, l2 return l1 = l2 with
+  | succ0, succ0 => eq_refl
+  | succS l1', _ =>
+    Empty_set_ind (fun _ => succS l1' = l2) l1'
+  | _, succS l2' =>
+    Empty_set_ind (fun _ => succ0 = succS l2') l2'
+  end.
+
+Fixpoint level_dec {N} :
+  forall (l1 : level N) (l2 : level N),
+    {l1 = l2} + {l1 <> l2} :=
+  match N return
+        forall (l1 : level N) (l2 : level N),
+          {l1 = l2} + {l1 <> l2}
+  with
+  | 0 =>
+    fun (l1 : level 0) l2 =>
+      Empty_set_rec (fun l => {l = l2} + {l <> l2}) l1
+  | S N =>
+    fun l1 l2 =>
+      match l1 return {l1 = l2} + {l1 <> l2} with
+      | succ0 =>
+        match l2 return {succ0 = l2} + {succ0 <> l2} with
+        | succ0 => left eq_refl
+        | succS l2' => right (discriminate_level l2')
+        end
+      | succS l1' =>
+        match l2 return {lS l1' = l2} + {lS l1' <> l2} with
+        | succ0 =>
+          right (fun eql => discriminate_level l1' (eq_sym eql))
+        | succS l2' =>
+          match level_dec l1' l2' with
+          | left eql => left (f_equal lS eql)
+          | right neql =>
+            right (fun eql => neql (injective_succS l1' l2' eql))
+          end
+        end
+      end
+  end.
+
+Fixpoint shift_level {N}
+  : level (S N) -> level N -> level (S N) :=
+  match N return level (S N) -> level N -> level (S N) with
+  | 0 => fun l1 l2 => Empty_set_rec _ l2
+  | S _ =>
+    fun l1 l2 =>
+      match l1 with
+      | succ0 => lS l2
+      | succS l1' =>
+        match l2 with
+        | succ0 => level_extend l2
+        | succS l2' => lS (shift_level l1' l2')
+        end
+      end
+    end.
+Arguments shift_level {N} l1 l2 : simpl nomatch.
+
+Fixpoint unshift_level {N} :
+  level N -> level (S N) -> level N :=
+  match N return level N -> level (S N) -> level N with
+  | 0 => fun l1 => Empty_set_rec _ l1
+  | S N' =>
+    fun l1 l2 =>
+      match l1, l2 with
+      | _, succ0 => l0
+      | succ0, succS l2' => l2'
+      | succS l1, succS l2 => lS (unshift_level l1 l2)
+      end
+  end.
+Arguments unshift_level {N} l1 l2 : simpl nomatch, rename.
+
+Definition pred_level {N} :
+  level (S (S N)) -> level (S N) :=
+  fun l =>
+    match l with
+    | succ0 => succ0
+    | succS l => l
+    end.
+
+Fixpoint unshift_level_neq {N} :
+  forall (l1 : level (S N)) (l2 : level (S N)),
+    l1 <> l2 -> level N :=
+  match N return
+        forall (l1 : level (S N)) (l2 : level (S N)),
+          l1 <> l2 -> level N
+  with
+  | 0 =>
+    fun l1 l2 neq => False_rec _ (neq level_one_eq)
+  | S N =>
+    fun l1 l2 =>
+      match l1, l2 return l1 <> l2 -> level (S N) with
+      | _, succ0 => fun _ => succ0
+      | succ0, succS l2' => fun _ => l2'
+      | succS l1, succS l2 =>
+        fun neq =>
+          lS (unshift_level_neq l1 l2
+                (fun eq => neq (f_equal succS eq)))
+      end
+  end.
+
+Arguments unshift_level {N} l1 l2 : simpl nomatch, rename.
+
+Definition cycle_in_level {N} :=
+  match N return level N -> morph level N level N with
+  | 0 => fun l => Empty_set_rec _ l
+  | S N =>
+    fun l1 V l2 =>
+      match l2 with
+      | succ0 => level_extend_by V l1
+      | succS l2 => shift_level (level_extend_by V l1) l2
+      end
+  end.
+Arguments cycle_in_level {N} l1 {V} l2 : simpl nomatch.
+
+Definition cycle_out_level {N} :=
+  match N return level N -> morph level N level N with
+  | 0 => fun l => Empty_set_rec _ l
+  | S N' =>
+    fun l1 V l2 =>
+      if level_dec (level_extend_by V l1) l2 then l0
+      else (unshift_level (level_extend_by V l1) (lS l2))
+  end.
+Arguments cycle_out_level {N} l1 {V} l2 : simpl nomatch.
 
 (* Variables are either free names or bound levels *)
 
@@ -119,40 +287,294 @@ Definition weak_var : morph var 0 var 1 :=
     end.
 Arguments weak_var {V} v : simpl nomatch.
 
-(* Algebra of operations on [var 0] *)
+Definition cycle_in_var {N} (l : level N) : morph var N var N :=
+  fun V v =>
+    match v with
+    | free n => free n
+    | bound l2 => bound (cycle_in_level l l2)
+    end.
+Arguments cycle_in_var {N} l {V} v : simpl nomatch.
 
-Inductive renaming (term : nset) :=
-| r_id
-| r_shift (n : name) (r : renaming term)
-| r_rename (n1 : name) (r : renaming term) (n2 : name)
-| r_subst (t : term 0) (r : renaming term) (n : name).
+Definition cycle_out_var {N} (l : level N) : morph var N var N :=
+  fun V v =>
+    match v with
+    | free n => free n
+    | bound l2 => bound (cycle_out_level l l2)
+    end.
+Arguments cycle_out_var {N} l {V} v : simpl nomatch.
 
-Arguments r_id {term}.
-Arguments r_shift {term} n r.
-Arguments r_rename {term} n1 r n2.
-Arguments r_subst {term} t r n.
+Definition lift_morph_var {N M} (m : morph var M var N) :
+  morph var (S M) var (S N) :=
+  fun V v =>
+    match v with
+    | free n =>
+      match m V (free n) with
+      | free n => free n
+      | bound l => bound (lS l)
+      end
+    | bound succ0 => bound l0
+    | bound (succS l) =>
+      match m V (bound l) with
+      | free n => free n
+      | bound l => bound (lS l)
+      end
+    end.
 
-(* Left-hand sides of renamings *)
+(* Algebra of operations on [var] *)
 
-Inductive pop (term : nset) : Type :=
-| p_open : name -> pop term
-| p_bind : term 0 -> pop term.
-Arguments p_open {term} n.
-Arguments p_bind {term} t.
+Inductive pushes : nat -> nat -> Set :=
+| pushes_id : pushes 0 0
+| pushes_weak : forall N M,
+    level (S N) -> pushes N M -> pushes (S N) M
+| pushes_swap : forall N M,
+    level (S N) -> pushes N M -> level (S M) -> pushes (S N) (S M)
+| pushes_close : forall N M,
+    level (S N) -> pushes N M -> name -> pushes (S N) M.
 
-Definition r_pop_weak {term} (p : @pop term) r :=
-  match p with
-  | p_open n => @r_shift term n r
-  | p_bind _ => r
+Arguments pushes_weak {N} {M} l r.
+Arguments pushes_swap {N} {M} l1 r l2.
+Arguments pushes_close {N} {M} l r n.
+
+Fixpoint pushes_weak_n {N} : pushes N 0 :=
+  match N return pushes N 0 with
+  | 0 => pushes_id
+  | S N => pushes_weak l0 pushes_weak_n
   end.
-Arguments r_pop_weak {term} !p r.
 
-Definition r_pop_close {term} (p : @pop term) r n :=
-  match p with
-  | p_open n2 => @r_rename term n2 r n
-  | p_bind t => r_subst t r n
+Fixpoint pushes_weakening {N M} : pushes (N + M) N :=
+  match N return pushes (N + M) N with
+  | 0 => pushes_weak_n
+  | S N => pushes_swap l0 pushes_weakening l0
   end.
-Arguments r_pop_close {term} !p r n.
+
+Fixpoint pushes_id_n {N} : pushes N N :=
+  match N return pushes N N with
+  | 0 => pushes_id
+  | S N => pushes_swap l0 pushes_id_n l0
+  end.
+
+Inductive static_renaming (N : nat) : nat -> Set :=
+| static_renaming_pushes : forall M, pushes N M -> static_renaming N M
+| static_renaming_shift : forall M,
+    name -> static_renaming N M -> static_renaming N M
+| static_renaming_open : forall M,
+    name -> static_renaming N M -> level (S M) ->
+    static_renaming N (S M)
+| static_renaming_rename : forall M,
+    name -> static_renaming N M -> name -> static_renaming N M.
+
+Arguments static_renaming_pushes {N} {M} r.
+Arguments static_renaming_shift {N} {M} n r.
+Arguments static_renaming_open {N} {M} n r l.
+Arguments static_renaming_rename {N} {M} n1 r n2.
+
+Definition static_renaming_id :=
+  static_renaming_pushes pushes_id.
+
+Fixpoint static_renaming_weak {N M}
+         (l : level (S N)) (r : static_renaming N M) :
+  static_renaming (S N) M :=
+  match r in static_renaming _ M
+        return static_renaming (S N) M
+  with
+  | static_renaming_pushes r =>
+    static_renaming_pushes (pushes_weak l r)
+  | static_renaming_shift n r =>
+    static_renaming_shift n (static_renaming_weak l r)
+  | @static_renaming_open _ M n r l' =>
+    static_renaming_open n (static_renaming_weak l r) l'
+  | static_renaming_rename n1 r n2 =>
+    static_renaming_rename n1 (static_renaming_weak l r) n2
+  end.
+
+Fixpoint static_renaming_swap {N M}
+         (l1 : level (S N)) (r : static_renaming N M) :
+  level (S M) -> static_renaming (S N) (S M) :=
+  match r in static_renaming _ M
+        return level (S M) -> static_renaming (S N) (S M)
+  with
+  | static_renaming_pushes r =>
+    fun l2 => static_renaming_pushes (pushes_swap l1 r l2)
+  | static_renaming_shift n r =>
+    fun l2 => static_renaming_shift n (static_renaming_swap l1 r l2)
+  | @static_renaming_open _ M n r l =>
+    fun l2 =>
+      static_renaming_open
+        n (static_renaming_swap l1 r (unshift_level l l2))
+        (shift_level l2 l)
+  | static_renaming_rename n1 r n2 =>
+    fun l2 =>
+      static_renaming_rename n1 (static_renaming_swap l1 r l2) n2
+  end.
+
+Fixpoint static_renaming_close {N M}
+         (l : level (S N)) (r : static_renaming N M) (n : name) :
+  static_renaming (S N) M :=
+  match r in static_renaming _ M
+        return static_renaming (S N) M
+  with
+  | static_renaming_pushes r =>
+    static_renaming_pushes (pushes_close l r n)
+  | static_renaming_shift n' r =>
+    static_renaming_shift n' (static_renaming_close l r n)
+  | @static_renaming_open _ M n' r l' =>
+    static_renaming_open n' (static_renaming_close l r n) l'
+  | static_renaming_rename n1 r n2 =>
+    static_renaming_rename
+      n1 (static_renaming_close l r (unshift_name n2 n))
+      (shift_name n n2)
+  end.
+
+Fixpoint apply_pushes_var {N M} (r : pushes N M)
+  : morph var M var N :=
+  match r in pushes N M return morph var M var N with
+  | pushes_id => morph_id
+  | @pushes_weak N M l r =>
+      (@cycle_out_var (S N) l)
+      @ lift_morph_var (apply_pushes_var r)
+      @ morph_extend_by M (@weak_var)
+  | @pushes_swap N M l1 r l2 =>
+        (@cycle_out_var (S N) l1)
+      @ lift_morph_var (apply_pushes_var r)
+      @ @cycle_in_var (S M) l2
+  | @pushes_close N M l r n =>
+        (@cycle_out_var (S N) l)
+      @ lift_morph_var (apply_pushes_var r)
+      @ morph_extend_by M (@close_var n)
+  end.
+
+Fixpoint apply_static_renaming_var {N M}
+         (r : static_renaming N M)
+  : morph var M var N :=
+  match r in static_renaming _ M
+        return morph var M var N with
+  | static_renaming_pushes r => apply_pushes_var r
+  | @static_renaming_shift _ M n r =>
+      morph_extend_by N (@open_var n)
+      @ lift_morph_var (apply_static_renaming_var r)
+      @ morph_extend_by M (@weak_var)
+  | @static_renaming_open _ M n r l =>
+      morph_extend_by N (@open_var n)
+      @ lift_morph_var (apply_static_renaming_var r)
+      @ @cycle_in_var (S M) l
+  | @static_renaming_rename _ M n1 r n2 =>
+      morph_extend_by N (@open_var n1)
+      @ lift_morph_var (apply_static_renaming_var r)
+      @ morph_extend_by M (@close_var n2)
+  end.
+
+Inductive pushes_rhs : nat -> nat -> Set :=
+| pushes_rhs_weak : forall N M,
+    pushes N M -> pushes_rhs (S N) M
+| pushes_rhs_swap : forall N M,
+    pushes N M -> level (S M) -> pushes_rhs (S N) (S M)
+| pushes_rhs_close : forall N M,
+    pushes N M -> name -> pushes_rhs (S N) M.
+
+Arguments pushes_rhs_weak {N} {M} r.
+Arguments pushes_rhs_swap {N} {M} r l.
+Arguments pushes_rhs_close {N} {M} r n.
+
+Definition pushes_rhs_add_weak {N M} (r : pushes_rhs N M)
+  : level N -> pushes_rhs (S N) M :=
+  match r in pushes_rhs N M
+        return level N -> pushes_rhs (S N) M with
+  | pushes_rhs_weak r =>
+    fun l1 => pushes_rhs_weak (pushes_weak l1 r)
+  | pushes_rhs_swap r l =>
+    fun l1 => pushes_rhs_swap (pushes_weak l1 r) l
+  | pushes_rhs_close r n =>
+    fun l1 => pushes_rhs_close (pushes_weak l1 r) n
+  end.
+
+Definition pushes_rhs_add_swap {N M} (r : pushes_rhs N M)
+  : level N -> level (S M) -> pushes_rhs (S N) (S M) :=
+  match r in pushes_rhs N M
+        return level N -> level (S M) -> pushes_rhs (S N) (S M) with
+  | pushes_rhs_weak r =>
+    fun l1 l2 => pushes_rhs_weak (pushes_swap l1 r l2)
+  | pushes_rhs_swap r l =>
+    fun l1 l2 =>
+      pushes_rhs_swap (pushes_swap l1 r (unshift_level l l2))
+                      (shift_level l2 l)
+  | pushes_rhs_close r n =>
+    fun l1 l2 => pushes_rhs_close (pushes_swap l1 r l2) n
+  end.
+
+Definition pushes_rhs_add_close {N M} (r : pushes_rhs N M)
+  : level N -> name -> pushes_rhs (S N) M :=
+  match r in pushes_rhs N M
+        return level N -> name -> pushes_rhs (S N) M with
+  | pushes_rhs_weak r =>
+    fun l1 n1 => pushes_rhs_weak (pushes_close l1 r n1)
+  | pushes_rhs_swap r l =>
+    fun l1 n1 => pushes_rhs_swap (pushes_close l1 r n1) l
+  | pushes_rhs_close r n =>
+    fun l1 n1 =>
+      pushes_rhs_close (pushes_close l1 r (unshift_name n n1))
+                       (shift_name n1 n)
+  end.
+
+Fixpoint transpose_level_pushes {N M}
+         (r : pushes N M) : level N -> pushes_rhs N M :=
+  match r in pushes N M return level N -> pushes_rhs N M with
+  | pushes_id => fun l => Empty_set_rec _ l
+  | pushes_weak l1 r =>
+    fun l =>
+      if level_dec l l1 then pushes_rhs_weak r
+      else
+        pushes_rhs_add_weak
+          (transpose_level_pushes r (unshift_level l1 l))
+          (unshift_level l l1) r
+  | pushes_swap l1 r l2 =>
+    fun l =>
+      if level_dec l l1 then pushes_rhs_swap r l2
+      else
+        pushes_rhs_add_swap
+          (transpose_level_pushes r (unshift_level l1 l))
+          (unshift_level l l1) r l2
+  | pushes_close l1 r n =>
+    fun l =>
+      if level_dec l l1 then pushes_rhs_close r n
+      else
+        pushes_rhs_add_close
+          (transpose_level_pushes r (unshift_level l1 l))
+          (unshift_level l l1) r n
+  end.
+
+Fixpoint transpose_level_pushes_left {N M}
+         (l : level N) (r : pushes N M) :=
+  match r with
+  | pushes_id => pushes_id
+  | pushes_weak l2 r =>
+      if level_dec l l2 then r
+      else transpose_level
+
+Fixpoint compose_pushes {N M O}
+         (r1 : pushes O N) (r2 : pushes N M) : pushes O M :=
+  match r1 with
+  | pushes_id => r2
+  | pushes_weak l r1 =>
+    pushes_weak l (compose_pushes r1 r2)
+  | pushes_swap l1 r1 l2 =>
+    
+  | pushes_close l r1 n =>
+
+
+
+Inductive renaming (term : nset) (N : nat) : nat -> Set :=
+| renaming_static : forall M, static_renaming N M -> renaming term N M
+| renaming_bind : forall M,
+    term N -> renaming term N M -> level (S M) ->
+    renaming term N (S M)
+| renaming_subst : forall M,
+    term N -> renaming term N M -> name -> renaming term N M.
+
+Arguments renaming_static {term} {N} {M} r.
+Arguments renaming_bind {term} {N} {M} t r l.
+Arguments renaming_subst {term} {N} {M} t r n.
+
+(*
 
 Declare Scope ren_scope.
 Delimit Scope ren_scope with ren.
@@ -174,27 +596,4 @@ Notation "a <- b" := (r_rename a r_id b)
 Notation "u // a" := (r_subst u r_id a)
   (at level 47, left associativity) : ren_scope.
 
-Fixpoint static {term} (r : renaming term) : SProp :=
-  match r with
-  | r_id => sUnit
-  | r_shift b r => static r
-  | r_rename b r a => static r
-  | r_subst u r a => sEmpty
-  end.
-
-Fixpoint apply_renaming_var {term} (r : renaming term)
-  : static r -> morph var 0 var 0 :=
-  match r return static r -> morph var 0 var 0 with
-  | r_id => fun _ => morph_id
-  | r_shift n r =>
-    fun s =>
-      (@open_var n
-       @ morph_extend (apply_renaming_var r s)
-       @ @weak_var)%morph
-  | r_rename n1 r n2 =>
-    fun s =>
-      (@open_var n1
-       @ morph_extend (apply_renaming_var r s)
-       @ @close_var n2)%morph
-  | r_subst t r n => sEmpty_rect _
-  end.
+*)
